WIP: imp prelude

theories/Skeleton.v
@@ -126,26 +126,6 @@ Module Sk.
   (*** TODO: It might be nice if Sk.t also constitutes a resource algebra ***)
   (*** At the moment, List.app is not assoc/commutative. We need to equip RA with custom equiv. ***)
 
-  Definition load_mem (sk: t): Mem.t :=
-    Mem.mk
-      (fun blk ofs =>
-         do '(_, gd) <- (List.nth_error sk blk);
-         match gd with
-         | Gfun =>
-           None
-         | Gvar gv =>
-           if (dec ofs 0%Z) then Some (Vint gv) else None
-         end)
-      (*** TODO: This simplified model doesn't allow function pointer comparsion.
-           To be more faithful, we need to migrate the notion of "permission" from CompCert.
-           CompCert expresses it with "nonempty" permission.
-       ***)
-      (*** TODO: When doing so, I would like to extend val with "Vfid (id: gname)" case.
-           That way, I might be able to support more higher-order features (overriding, newly allocating function)
-       ***)
-      (List.length sk)
-  .
-
   Definition load_skenv (sk: t): (SkEnv.t) :=
     let n := List.length sk in
     {|
