mem/Mem0.v
@@ -94,7 +94,7 @@ Section PROOF.
     {|
       ModSem.fnsems := [("alloc", cfunU allocF) ; ("free", cfunU freeF) ; ("load", cfunU loadF) ; ("store", cfunU storeF) ; ("cmp", cfunU cmpF)];
       ModSem.mn := "Mem";
-      ModSem.initial_st := (Sk.load_mem sk)↑;
+      ModSem.initial_st := (Mem.load_mem sk)↑;
     |}
   .
 
